Moving to seq in IntStore

examples/dm4free/FStar.DM4F.IntStore.fst
@@ -1,8 +1,9 @@
 module FStar.DM4F.IntStore
 
-open FStar.DM4F.IntStoreAux
+(* open FStar.DM4F.IntStoreAux *)
+open FStar.Seq
 
-type int_store (a:Type) = list int -> M (option a * list int)
+type int_store (a:Type) = seq int -> M (option a * seq int)
 let return_is (a:Type) (x:a) : int_store a = fun store -> Some x, store
 let bind_is (a b : Type) (x:int_store a) (f: a -> int_store b) : int_store b =
   fun store ->
@@ -11,7 +12,7 @@ let bind_is (a b : Type) (x:int_store a) (f: a -> int_store b) : int_store b =
     | None -> None, store'
     | Some xa -> f xa store'
 
-let get () : int_store (list int) = fun store -> Some store, store
+let get () : int_store (seq int) = fun store -> Some store, store
 let put s : int_store unit = fun _ -> Some (), s
 let raise_impl () : int_store False = fun store -> None, store
 
@@ -26,35 +27,36 @@ total reifiable reflectable new_effect_for_free {
      ; raise_ = raise_impl
 }
 
-effect IntStore (a:Type) (pre:INT_STORE?.pre) (post: list int -> option a -> list int -> GTot Type0) =
+effect IntStore (a:Type) (pre:INT_STORE?.pre) (post: seq int -> option a -> seq int -> GTot Type0) =
   INT_STORE a (fun l0 p -> pre l0 /\ (forall x l1. pre l0 /\ post l0 x l1 ==> p (x, l1)))
 
 effect IS (a:Type) =
-  INT_STORE a (fun (l0:list int) (p:((option a * list int) -> Type0)) -> forall (x:(option a * list int)). p x)
+  INT_STORE a (fun (l0:seq int) (p:((option a * seq int) -> Type0)) -> forall (x:(option a * seq int)). p x)
 
 let raise_ (#a:Type) ()
   : IntStore a (fun _ -> True) (fun l0 x l1 -> l0 == l1 /\ None? x)
 = let x = INT_STORE?.raise_ () in begin match x with end
 
 reifiable
-let read (r:index) =
-  let store = INT_STORE?.get () in
-  match nth_opt r store with
-  | None -> raise_ ()
-  | Some x -> x
+let read (i:nat) =
+  let store = IS?.get () in
+  if i < length store
+  then index store i
+  else raise_
 
 reifiable
-let write (r:index) (x:int) =
-  let store = INT_STORE?.get () in
-  match set_nth_opt [] r store x with
-  | None -> raise_ ()
-  | Some store' -> INT_STORE?.put store'
+let write (r:nat) (x:int) =
+  let store = IS?.get () in
+  if i < length store
+  then IS?.put (upd store i x)
+  else raise_ ()
 
 
-(* let total_read_lemma (store:list int) (r:index) *)
-(*   : Lemma (r `in_` store ==> Some? (fst (reify (read r) store))) *)
-(* = () *)
 
-(* let total_write_lemma (store:list int) (r:index) (x:int) *)
-(*   : Lemma (r `in_` store ==> Some? (fst (reify (write r x) store))) *)
-(* = () *)
+let total_read_lemma (store:seq int) (r:index)
+  : Lemma (requires r < length store) (ensures Some? (fst (reify (read r) store)))
+= ()
+
+let total_write_lemma (store:seq int) (r:index) (x:int)
+  : Lemma (requires r < length store) (ensures Some? (fst (reify (write r x) store)))
+= ()
